Simplify and update
- evmap is dropped
- per-item invariant is implemented with inv-in-inv
- peritem.v is simplified by proving an ad-hoc iter spec
- update to latest iris
- related fixes

theories/flat.v
@@ -1,12 +1,11 @@
 (* Flat Combiner *)
-
 From iris.program_logic Require Export weakestpre.
 From iris.heap_lang Require Export lang.
 From iris.heap_lang Require Import proofmode notation.
 From iris.heap_lang.lib Require Import spin_lock.
 From iris.algebra Require Import auth frac agree excl agree gset gmap.
 From iris.base_logic Require Import big_op saved_prop.
-From iris_atomic Require Import misc peritem sync evmap.
+From iris_atomic Require Import misc peritem sync.
 
 Definition doOp : val :=
   λ: "p",
@@ -49,24 +48,20 @@ Definition mk_flat : val :=
 
 Definition reqR := prodR fracR (agreeR valC). (* request x should be kept same *)
 Definition toks : Type := gname * gname * gname * gname * gname. (* a bunch of tokens to do state transition *)
-Definition tokmR : ucmraT := evmapR loc toks unitR. (* tie each slot to tokens *)
 Class flatG Σ := FlatG {
   req_G :> inG Σ reqR;
-  tok_G :> inG Σ (authR tokmR);
   sp_G  :> savedPropG Σ (ofe_funCF val idCF)
 }.
 
 Definition flatΣ : gFunctors :=
   #[ GFunctor (constRF reqR);
-     GFunctor (constRF (authR tokmR));
-     savedPropΣ (ofe_funCF val idCF)
-   ].
+     savedPropΣ (ofe_funCF val idCF) ].
 
 Instance subG_flatΣ {Σ} : subG flatΣ Σ → flatG Σ.
-Proof. intros [?%subG_inG [?%subG_inG [? _]%subG_inv]%subG_inv]%subG_inv. split; apply _. Qed.
+Proof. intros [?%subG_inG [? _]%subG_inv]%subG_inv. split; apply _. Qed.
 
 Section proof.
-  Context `{!heapG Σ, !lockG Σ, !evidenceG loc val unitR Σ, !flatG Σ} (N : namespace).
+  Context `{!heapG Σ, !lockG Σ, !flatG Σ} (N: namespace).
 
   Definition init_s (ts: toks) :=
     let '(_, γ1, γ3, _, _) := ts in (own γ1 (Excl ()) ∗ own γ3 (Excl ()))%I.
@@ -86,61 +81,32 @@ Section proof.
     (∃ Q: val → val → iProp Σ,
        own γx ((1/2)%Qp, to_agree x) ∗ saved_prop_own γq (Q x) ∗
        Q x y ∗ own γ1 (Excl ()) ∗ own γ4 (Excl ()))%I.
-
-  Definition evm := ev loc toks.
   
-  (* p slot invariant *)
-  Definition p_inv R (γm γr: gname) (v: val) :=
-    (∃ (ts: toks) (p : loc),
-       ⌜v = #p⌝ ∗ evm γm p ts ∗
-       ((* INIT *)
-        (∃ y: val, p ↦{1/2} InjRV y ∗ init_s ts)∨
-        (* INSTALLED *)
-        (∃ f x: val, p ↦{1/2} InjLV (f, x) ∗ installed_s R ts f x) ∨
-        (* RECEIVED *)
-        (∃ f x: val, p ↦{1/2} InjLV (f, x) ∗ received_s ts x γr) ∨
-        (* FINISHED *)
-        (∃ x y: val, p ↦{1/2} InjRV y ∗ finished_s ts x y)))%I.
+  Definition p_inv R (γm γr: gname) (ts: toks) (p : loc) :=
+    ( (* INIT *)
+      (∃ y: val, p ↦ InjRV y ∗ init_s ts) ∨
+      (* INSTALLED *)
+      (∃ f x: val, p ↦ InjLV (f, x) ∗ installed_s R ts f x) ∨
+      (* RECEIVED *)
+      (∃ f x: val, p ↦ InjLV (f, x) ∗ received_s ts x γr) ∨
+      (* FINISHED *)
+      (∃ x y: val, p ↦ InjRV y ∗ finished_s ts x y))%I.
 
-  Definition srv_stack_inv R γs γm γr s := (∃ xs, is_stack' (p_inv R γm γr) γs xs s)%I.
+  Definition p_inv' R γm γr : val → iProp Σ :=
+    (λ v: val, ∃ ts (p: loc), ⌜v = #p⌝ ∗ inv N (p_inv R γm γr ts p))%I.
 
-  Definition srv_tokm_inv γm := (∃ m : tokmR, own γm (● m) ∗ [∗ map] p ↦ _ ∈ m, ∃ v, p ↦{1/2} v)%I.
-
-  Lemma install_push_spec R
-        (p: loc) (γs γm γr: gname) (ts: toks)
-        (s: loc) (f x: val) (Φ: val → iProp Σ) :
-    inv N (srv_stack_inv R γs γm γr s ∗ srv_tokm_inv γm) ∗
-    evm γm p ts ∗ installed_s R ts f x ∗
-    p ↦{1/2} InjLV (f, x) ∗ ((∃ hd, evs γs hd #p) -∗ Φ #())
-    ⊢ WP push #s #p {{ Φ }}.
-  Proof.
-    iIntros "(#? & Hpm & Hs & Hp & HΦ)".
-    rewrite /srv_stack_inv.
-    iDestruct (push_spec N (p_inv R γm γr) (fun v => (∃ hd, evs γs hd #p) ∗ ⌜v = #()⌝)%I
-               with "[-HΦ]") as "Hpush"=>//.
-    - iSplitL "Hp Hs Hpm"; last eauto.
-      iExists ts. iExists p. iSplit=>//. iFrame "Hpm".
-      iRight. iLeft. iExists f, x. iFrame.
-    - iApply wp_wand_r.
-      iSplitL "Hpush"; first done.
-      iIntros (?) "[? %]". subst.
-      by iApply "HΦ".
-  Qed.
+  Definition srv_bag R γm γr s := (∃ xs, is_bag_R N (p_inv' R γm γr) xs s)%I.
 
   Definition installed_recp (ts: toks) (x: val) (Q: val → iProp Σ) :=
     let '(γx, _, γ3, _, γq) := ts in
     (own γ3 (Excl ()) ∗ own γx ((1/2)%Qp, to_agree x) ∗ saved_prop_own γq Q)%I.
 
-  Lemma install_spec
-        R P Q
-        (f x: val) (γs γm γr: gname) (s: loc)
-        (Φ: val → iProp Σ):
-    inv N (srv_stack_inv R γs γm γr s ∗ srv_tokm_inv γm) ∗
-    P ∗ ({{ R ∗ P }} f x {{ v, R ∗ Q v }}) ∗
-    (∀ (p: loc) (ts: toks), installed_recp ts x Q -∗ evm γm p ts -∗(∃ hd, evs γs hd #p) -∗ Φ #p)
-    ⊢ WP install f x #s {{ Φ }}.
+  Lemma install_spec R P Q (f x: val) (γm γr: gname) (s: loc):
+    {{{ inv N (srv_bag R γm γr s) ∗ P ∗ ({{ R ∗ P }} f x {{ v, R ∗ Q v }}) }}}
+      install f x #s
+    {{{ p ts, RET #p; installed_recp ts x Q ∗ inv N (p_inv R γm γr ts p) }}}.
   Proof.
-    iIntros "(#? & Hpx & Hf & HΦ)".
+    iIntros (Φ) "(#? & HP & Hf) HΦ".
     wp_seq. wp_let. wp_let. wp_alloc p as "Hl".
     iApply fupd_wp.
     iMod (own_alloc (Excl ())) as (γ1) "Ho1"; first done.
@@ -148,145 +114,73 @@ Section proof.
     iMod (own_alloc (Excl ())) as (γ4) "Ho4"; first done.
     iMod (own_alloc (1%Qp, to_agree x)) as (γx) "Hx"; first done.
     iMod (saved_prop_alloc (F:=(ofe_funCF val idCF)) Q) as (γq) "#?".
-    iInv N as "[Hrs >Hm]" "Hclose".
-    iDestruct "Hm" as (m) "[Hm HRm]".
-    destruct (m !! p) eqn:Heqn.
-    - (* old name *)
-      iDestruct (big_sepM_delete (fun p _ => ∃ v : val, p ↦{1 / 2} v)%I m with "HRm") as "[Hp HRm]"=>//.
-      iDestruct "Hp" as (?) "Hp". iExFalso. iApply bogus_heap; last by iFrame "Hl Hp". auto.
-    - (* fresh name *)
-      iDestruct (evmap_alloc _ _ _ m p (γx, γ1, γ3, γ4, γq) with "[Hm]") as ">[Hm1 #Hm2]"=>//.
-      iDestruct "Hl" as "[Hl1 Hl2]".
-      iMod ("Hclose" with "[HRm Hm1 Hl1 Hrs]").
-      + iNext. iFrame. iExists (<[p := (∅, DecAgree (γx, γ1, γ3, γ4, γq))]> m). iFrame.
-        iDestruct (big_sepM_insert _ m with "[-]") as "H"=>//.
-        iSplitL "Hl1"; last by iAssumption. eauto.
-      + iDestruct (own_update with "Hx") as ">[Hx1 Hx2]"; first by apply pair_l_frac_op_1'.
-        iModIntro. wp_let. wp_bind ((push _) _).
-        iApply install_push_spec=>//.
-        iFrame "#". rewrite /evm /installed_s. iFrame.
-        iSplitL "Hpx Hf".
-        { (* TODO: Something somewhere can be simplified so that we don't have
-             to add these dummy arguments any more. *)
-          iExists (fun _ => P), (fun _ => Q). by iFrame. }
-        iIntros "Hhd". wp_seq. 
-        iSpecialize ("HΦ" $! p (γx, γ1, γ3, γ4, γq) with "[-Hhd]")=>//.
-        { rewrite /installed_recp. iFrame. iFrame "#". }
-        by iApply ("HΦ" with "[]").
+    iDestruct (own_update with "Hx") as ">[Hx1 Hx2]"; first by apply pair_l_frac_op_1'.
+    iModIntro. wp_let. wp_bind (push _ _).
+    iMod (inv_alloc N _ (p_inv R γm γr (γx, γ1, γ3, γ4, γq) p)
+          with "[-HΦ Hx2 Ho3]") as "#HRx"; first eauto.
+    { iNext. iRight. iLeft. iExists f, x. iFrame.
+      iExists (λ _, P), (λ _ v, Q v).
+      iFrame. iFrame "#". }
+    iApply (push_spec N (p_inv' R γm γr) s #p
+            with "[-HΦ Hx2 Ho3]")=>//.
+    { iFrame "#". iExists (γx, γ1, γ3, γ4, γq), p.
+      iSplitR; first done. iFrame "#". }
+    iNext. iIntros "?".
+    wp_seq. iApply ("HΦ" $! p (γx, γ1, γ3, γ4, γq)).
+    iFrame. iFrame "#".
   Qed.
 
-  Lemma loop_iter_doOp_spec R (s hd: loc) (γs γm γr: gname) xs Φ:
-    inv N (srv_stack_inv R γs γm γr s ∗ srv_tokm_inv γm) ∗ own γr (Excl ()) ∗ R ∗
-    is_list' γs hd xs ∗ (own γr (Excl ()) -∗ R -∗ Φ #())
-    ⊢ WP iter #hd doOp {{ Φ }}.
+  Definition f_spec (R: iProp Σ) (f: val) (Rf: iProp Σ) x :=
+    {{{ inv N R ∗ Rf }}}
+      f x
+    {{{ RET #(); Rf }}}.
+
+  Lemma doOp_f_spec R γm γr (p: loc) ts:
+    f_spec (p_inv R γm γr ts p) doOp (own γr (Excl ()) ∗ R)%I #p.
   Proof.
-    iIntros "(#? & Ho2 & HR & Hlist' & HΦ)".
-    iApply (iter_spec N (p_inv R γm γr) Φ
-                      (* (fun v => v = #() ∗ own γr (Excl ()) ∗ R)%I *)
-                      γs s (own γr (Excl ()) ∗ R)%I (srv_tokm_inv γm) xs hd doOp doOp
-            with "[-]")=>//.
-    - rewrite /f_spec.
-      iIntros (Φ' x) "(#? & Hev & [Hor HR] & HΦ')".
-      iDestruct "Hev" as (xhd) "#Hev".
-      wp_rec.  wp_bind (! _)%E. iInv N as "[Hs >Hm]" "Hclose".
-      iDestruct "Hs" as (gxs ghd) "[>Hghd [>Hgxs HRs]]". (* global xs, hd *)
-      iDestruct "HRs" as (m) "[>Hom HRs]".
-      (* acccess *)
-      iDestruct (ev_map_witness _ _ _ m with "[Hev Hom]") as %H'; first by iFrame.
-      iDestruct (big_sepM_delete_later (perR _) m with "HRs") as "[Hp HRm]"=>//.
-      iDestruct "Hp" as (v') "[>% [Hpinv' >Hahd]]". inversion H. subst.
-      iDestruct "Hpinv'" as (ts p'') "[>% [>#Hevm [Hp | [Hp | [Hp | Hp]]]]]"; subst.
-      + iDestruct "Hp" as (y) "(>Hp & Hs)".
-        wp_load. iMod ("Hclose" with "[-Hor HR Hev HΦ']").
-        { iNext. iFrame. iExists gxs, ghd.
-          iFrame "Hghd Hgxs". iExists m.
-          iFrame "Hom". iDestruct (big_sepM_delete _ m with "[-]") as "?"=>//.
-          iFrame. iExists #p''. iSplitR; first done. iExists ts, p''.
-          iSplitR; first done. iFrame "#". iLeft. iExists y. iFrame. }
-        iModIntro. wp_match. iApply ("HΦ'" with "[Hor HR]"). iFrame.
-      + iDestruct "Hp" as (f' x') "(Hp & Hs)".
-        wp_load. destruct ts as [[[[γx γ1] γ3] γ4] γq].
-        iDestruct "Hs" as (P Q) "(Hx & Hpx & Hf' & HoQ & Ho1 & Ho4)".
-        iAssert (|==> own γx (((1/2/2)%Qp, to_agree x') ⋅
-                               ((1/2/2)%Qp, to_agree x')))%I with "[Hx]" as ">[Hx1 Hx2]".
-        { iDestruct (own_update with "Hx") as "?"; last by iAssumption.
-          rewrite -{1}(Qp_div_2 (1/2)%Qp).
-          by apply pair_l_frac_op'. }
-        iMod ("Hclose" with "[-Hf' Ho1 Hx2 HR HoQ HΦ' Hpx]").
-        { iNext. iFrame. iExists gxs, ghd.
-          iFrame "Hghd Hgxs". iExists m.
-          iFrame "Hom". iDestruct (big_sepM_delete _ m with "[-]") as "?"=>//.
-          simpl. iFrame. iExists #p''. iSplitR; auto. rewrite /allocated.
-          iExists (γx, γ1, γ3, γ4, γq), p''. iSplitR; auto.
-          iFrame "#". iRight. iRight. iLeft. iExists f', x'. iFrame. }
-        iModIntro. wp_match.
-        wp_proj. wp_proj.
-        wp_bind (f' _). iApply wp_wand_r. iSplitL "Hpx Hf' HR".
-        { iApply "Hf'". iFrame. }
-        iIntros (v) "[HR HQ]".
-        wp_value. iInv N as "[Hs >Hm]" "Hclose".
-        iDestruct "Hs" as (xs'' hd''') "[>Hhd [>Hxs HRs]]".
-        iDestruct "HRs" as (m') "[>Hom HRs]".
-        iDestruct (ev_map_witness _ _ _ m' with "[Hevm Hom]") as %?; first by iFrame.
-        iDestruct (big_sepM_delete_later (perR _) m' with "HRs") as "[Hp HRm]"=>//.
-        iDestruct "Hp" as (v'') "[>% [Hpinv' >Hhd'']]". inversion H1. subst.
-        iDestruct "Hpinv'" as ([[[[γx' γ1'] γ3'] γ4'] γq'] p'''') "[>% [>#Hevm2 Hps]]".
-        inversion H2. subst.
-        destruct (decide (γ1 = γ1' ∧ γx = γx' ∧ γ3 = γ3' ∧ γ4 = γ4' ∧ γq = γq'))
-          as [[? [? [? [? ?]]]]|Hneq]; subst.
-        {
-          iDestruct "Hps" as "[Hp | [Hp | [Hp | Hp]]]".
-          * iDestruct "Hp" as (?) "(_ & >Ho1' & _)".
-            iApply excl_falso. iFrame.
-          * iDestruct "Hp" as (? ?) "[>? Hs]". iDestruct "Hs" as (? ?) "(_ & _ & _ & _ & >Ho1' & _)".
-            iApply excl_falso. iFrame.
-          * iDestruct "Hp" as (? x5) ">(Hp & Hx & Hor & Ho4)".
-            iDestruct "Hm" as (m2) "[Hom2 HRp]".
-            iDestruct (ev_map_witness _ _ _ m2 with "[Hevm Hom2]") as %?; first by iFrame.
-            iDestruct (big_sepM_delete _ m2 with "HRp") as "[HRk HRp]"=>//.
-            iDestruct "HRk" as (?) "HRk".
-            iDestruct (@mapsto_agree with "[$HRk $Hp]") as %->.
-            iCombine "HRk" "Hp" as "Hp". wp_store.
-            (* now close the invariant *)
-            iDestruct (m_frag_agree' with "[Hx Hx2]") as "[Hx %]"; first iFrame.
-            subst. rewrite Qp_div_2. iMod ("Hclose" with "[-HR Hor HΦ']").
-            { iNext. iDestruct "Hp" as "[Hp1 Hp2]".
-              iAssert (srv_tokm_inv γm) with "[Hp1 HRp Hom2]" as "HRp".
-              { iExists m2. iFrame. iApply (big_sepM_delete _ m2)=>//.
-                iFrame. eauto. }
-              (* FIXME: These iFrame are really slow. *)
-              iFrame. iExists xs''. iFrame. iExists hd'''. iFrame.
-              iExists m'. iFrame.
-              iDestruct (big_sepM_delete _ m' with "[-]") as "?"=>//.
-              { simpl. iFrame. iExists #p''''.
-                iSplitR; first auto. iExists (γx', γ1', γ3', γ4', γq'), p''''.
-                iSplitR; first auto. iFrame "Hevm". iRight. iRight.
-                iRight. iExists x5, v. iFrame.
-                iExists Q. iFrame. 
-              }
-            }
-            iApply "HΦ'". iFrame.
-          * iDestruct "Hp" as (? ?) "[? Hs]". iDestruct "Hs" as (?) "(_ & _ & _ & >Ho1' & _)".
-            iApply excl_falso. iFrame.
-        }
-        { iDestruct (evmap_frag_agree_split with "[]") as "%"; first iFrame "Hevm Hevm2".
-          inversion H3. subst. by contradiction Hneq. }
-      + destruct ts as [[[[γx γ1] γ3] γ4] γq]. iDestruct "Hp" as (? x) "(_ & _ & >Ho2' & _)".
+    iIntros (Φ) "(#H1 & Hor & HR) HΦ".
+    wp_rec. wp_bind (! _)%E.
+    iInv N as "Hp" "Hclose".
+    iDestruct "Hp" as "[Hp | [Hp | [Hp | Hp]]]"; subst.
+    - iDestruct "Hp" as (y) "[>Hp Hts]".
+      wp_load. iMod ("Hclose" with "[-Hor HR HΦ]").
+      { iNext. iFrame "#". iLeft. iExists y. iFrame. }
+      iModIntro. wp_match. iApply ("HΦ" with "[Hor HR]"). iFrame.
+    - destruct ts as [[[[γx γ1] γ3] γ4] γq].
+      iDestruct "Hp" as (f x) "(>Hp & Hts)".
+      iDestruct "Hts" as (P Q) "(>Hx & Hpx & Hf' & HoQ & >Ho1 & >Ho4)".
+      iAssert (|==> own γx (((1/2/2)%Qp, to_agree x) ⋅
+                            ((1/2/2)%Qp, to_agree x)))%I with "[Hx]" as ">[Hx1 Hx2]".
+      { iDestruct (own_update with "Hx") as "?"; last by iAssumption.
+        rewrite -{1}(Qp_div_2 (1/2)%Qp).
+        by apply pair_l_frac_op'. }
+      wp_load. iMod ("Hclose" with "[-Hf' Ho1 Hx2 HoQ HR HΦ Hpx]").
+      { iNext. iFrame. iFrame "#". iRight. iRight. iLeft. iExists f, x. iFrame. }
+      iModIntro. wp_match. wp_proj. wp_proj.
+      wp_bind (f _). iApply wp_wand_r. iSplitL "Hpx Hf' HR".
+      { iApply "Hf'". iFrame. }
+      iIntros (v) "[HR HQ]". wp_value.
+      iInv N as "Hx" "Hclose".
+      iDestruct "Hx" as "[Hp | [Hp | [Hp | Hp]]]"; subst.
+      * iDestruct "Hp" as (?) "(_ & >Ho1' & _)".
         iApply excl_falso. iFrame.
-      + destruct ts as [[[[γx γ1] γ3] γ4] γq]. iDestruct "Hp" as (x' y) "[Hp Hs]".
+      * iDestruct "Hp" as (? ?) "[>? Hs]". iDestruct "Hs" as (? ?) "(_ & _ & _ & _ & >Ho1' & _)".
+        iApply excl_falso. iFrame.
+      * iDestruct "Hp" as (? x5) ">(Hp & Hx & Hor & Ho4)".
+        wp_store. iDestruct (m_frag_agree' with "[Hx Hx2]") as "[Hx %]"; first iFrame.
+        subst. rewrite Qp_div_2. iMod ("Hclose" with "[-HR Hor HΦ]").
+        { iNext. iDestruct "Hp" as "[Hp1 Hp2]". iRight. iRight.
+          iRight. iExists x5, v. iFrame. iExists Q. iFrame. }
+        iApply "HΦ". iFrame.
+      * iDestruct "Hp" as (? ?) "[? Hs]". iDestruct "Hs" as (?) "(_ & _ & _ & >Ho1' & _)".
+        iApply excl_falso. iFrame.
+    - destruct ts as [[[[γx γ1] γ3] γ4] γq]. iDestruct "Hp" as (? x) "(_ & _ & >Ho2' & _)".
+      iApply excl_falso. iFrame.
+    - destruct ts as [[[[γx γ1] γ3] γ4] γq]. iDestruct "Hp" as (x' y) "[Hp Hs]".
         iDestruct "Hs" as (Q) "(>Hx & HoQ & HQxy & >Ho1 & >Ho4)".
-        wp_load. iMod ("Hclose" with "[-HΦ' HR Hor]").
-        { iNext. iFrame. iExists gxs, ghd.
-          iFrame "Hghd Hgxs". iExists m.
-          iFrame "Hom". iDestruct (big_sepM_delete _ m with "[-]") as "?"=>//.
-          iFrame. iExists #p''. iSplitR; first auto. iExists (γx, γ1, γ3, γ4, γq), p''.
-          iSplitR; auto. iFrame "#". iRight. iRight. iRight. iExists x', y. iFrame.
-          iExists Q. iFrame. }
-        iModIntro. wp_match.
-        iApply "HΦ'". iFrame.
-    - apply to_of_val.
-    - iFrame "#". iFrame. iIntros "[Hor HR]".
-      iApply ("HΦ" with "Hor HR").
+        wp_load. iMod ("Hclose" with "[-HΦ HR Hor]").
+        { iNext. iRight. iRight. iRight. iExists x', y. iFrame. iExists Q. iFrame. }
+        iModIntro. wp_match. iApply "HΦ". iFrame.
   Qed.
 
   Definition own_γ3 (ts: toks) := let '(_, _, γ3, _, _) := ts in own γ3 (Excl ()).
@@ -294,122 +188,111 @@ Section proof.
     let '(γx, _, _, _, γq) := ts in
     (∃ Q, own γx ((1 / 2)%Qp, to_agree x) ∗ saved_prop_own γq (Q x) ∗ Q x y)%I.
 
-  Lemma try_srv_spec R (s: loc) (lk: val) (γs γr γm γlk: gname) Φ :
-    inv N (srv_stack_inv R γs γm γr s ∗ srv_tokm_inv γm) ∗
+  Lemma loop_iter_doOp_spec R (γm γr: gname) xs:
+  ∀ (hd: loc),
+    {{{ is_list_R N (p_inv' R γm γr) hd xs ∗ own γr (Excl ()) ∗ R }}}
+      iter #hd doOp
+    {{{ RET #(); own γr (Excl ()) ∗ R }}}.
+  Proof.
+    induction xs as [|x xs' IHxs].
+    - iIntros (hd Φ) "[Hxs ?] HΦ".
+      simpl. wp_rec. wp_value. wp_let.
+      iDestruct "Hxs" as (?) "Hhd".
+      wp_load. wp_match. by iApply "HΦ".
+    - iIntros (hd Φ) "[Hxs HRf] HΦ". simpl.
+      iDestruct "Hxs" as (hd' ?) "(Hhd & #Hinv & Hxs')".
+      wp_rec. wp_value. wp_let. wp_bind (! _)%E.
+      iInv N as "H" "Hclose".
+      iDestruct "H" as (ts p) "[>% #?]". subst.
+      wp_load. iMod ("Hclose" with "[]").
+      { iNext. iExists ts, p. eauto. }
+      iModIntro. wp_match. wp_proj. wp_bind (doOp _).
+      iDestruct (doOp_f_spec R γm γr p ts) as "Hf".
+      iApply ("Hf" with "[HRf]").
+      { iFrame. iFrame "#". }
+      iNext. iIntros "HRf".
+      wp_seq. wp_proj. iApply (IHxs with "[-HΦ]")=>//.
+      iFrame "#"; first by iFrame. eauto.
+  Qed.
+
+  Lemma try_srv_spec R (s: loc) (lk: val) (γr γm γlk: gname) Φ :
+    inv N (srv_bag R γm γr s) ∗
     is_lock N γlk lk (own γr (Excl ()) ∗ R) ∗ Φ #()
     ⊢ WP try_srv lk #s {{ Φ }}.
   Proof.
-    iIntros "(#? & #? & HΦ)".
-    wp_seq. wp_let.
+    iIntros "(#? & #? & HΦ)". wp_seq. wp_let.
     wp_bind (try_acquire _). iApply (try_acquire_spec with "[]"); first done.
     iNext. iIntros ([]); last by (iIntros; wp_if).
-    (* acquired the lock *)
     iIntros "[Hlocked [Ho2 HR]]".
     wp_if. wp_bind (! _)%E.
-    iInv N as "[H >Hm]" "Hclose".
-    iDestruct "H" as (xs' hd') "[>Hs [>Hxs HRs]]".
-    wp_load. iDestruct (dup_is_list' with "[Hxs]") as ">[Hxs1 Hxs2]"; first by iFrame.
-    iMod ("Hclose" with "[Hs Hxs1 HRs Hm]").
+    iInv N as "H" "Hclose".
+    iDestruct "H" as (xs' hd') "[>Hs Hxs]".
+    wp_load. iDestruct (dup_is_list_R with "[Hxs]") as ">[Hxs1 Hxs2]"; first by iFrame.
+    iMod ("Hclose" with "[Hs Hxs1]").
     { iNext. iFrame. iExists xs', hd'. by iFrame. }
-    iModIntro. wp_let.
-    wp_bind (iter _ _).
+    iModIntro. wp_let. wp_bind (iter _ _).
     iApply wp_wand_r. iSplitL "HR Ho2 Hxs2".
-    { iApply (loop_iter_doOp_spec R _ _ _ _ _ _ (fun v => own γr (Excl ()) ∗ R ∗ ⌜v = #()⌝))%I=>//.      
-      iFrame "#". iFrame. iIntros "? ?". by iFrame. }
-    iIntros (f') "[Ho [HR %]]". subst.
-    wp_let. iApply (release_spec with "[Hlocked Ho HR]"); first iFrame "#∗".
+    { iApply (loop_iter_doOp_spec R _ _ _ _ (λ _, own γr (Excl ()) ∗ R)%I with "[-]")=>//.
+      iFrame "#". iFrame. eauto. }
+    iIntros (f') "[Ho HR]". wp_seq.
+    iApply (release_spec with "[Hlocked Ho HR]"); first iFrame "#∗".
     iNext. iIntros. done.
   Qed.
 
   Lemma loop_spec R (p s: loc) (lk: val)
-        (γs γr γm γlk: gname) (ts: toks) Φ:
-    inv N (srv_stack_inv R γs γm γr s ∗ srv_tokm_inv γm) ∗
-    is_lock N γlk lk (own γr (Excl ()) ∗ R) ∗
-    own_γ3 ts ∗ evm γm p ts ∗
-    (∃ hd, evs γs hd #p) ∗ (∀ x y, finished_recp ts x y -∗ Φ y)
-    ⊢ WP loop #p #s lk {{ Φ }}.
+        (γs γr γm γlk: gname) (ts: toks):
+    {{{ inv N (srv_bag R γm γr s) ∗ inv N (p_inv R γm γr ts p) ∗
+        is_lock N γlk lk (own γr (Excl ()) ∗ R) ∗ own_γ3 ts }}}
+      loop #p #s lk
+    {{{ x y, RET y; finished_recp ts x y }}}.
   Proof.
-    iIntros "(#? & #? & Ho3 & #Hev & Hhd & HΦ)".
+    iIntros (Φ) "(#? & #? & #? & Ho3) HΦ".
     iLöb as "IH". wp_rec. repeat wp_let.
-    wp_bind (! _)%E. iInv N as "[Hinv >?]" "Hclose".
-    iDestruct "Hinv" as (xs hd) "[>Hs [>Hxs HRs]]".
-    iDestruct "HRs" as (m) "[>Hom HRs]".
-    iDestruct "Hhd" as (hdp) "Hhd".
-    destruct (m !! hdp) eqn:Heqn.
-    - iDestruct (big_sepM_delete_later _ m with "HRs") as "[Hp Hrs]"=>//.
-      iDestruct "Hp" as (?) "[>% [Hpr ?]]"; subst.
-      iDestruct "Hpr" as (ts' p') "(>% & >Hp' & Hp)".
-      subst. iDestruct (ev_map_witness _ _ _ m with "[Hom Hhd]") as %H=>//; first iFrame.
-      rewrite Heqn in H. inversion H. subst.
-      iDestruct (evmap_frag_agree_split with "[Hp']") as "%"; first iFrame "Hev Hp'". subst.
-      destruct ts' as [[[[γx γ1] γ3] γ4] γq].
-      iDestruct "Hp" as "[Hp | [Hp | [ Hp | Hp]]]".
-      + iDestruct "Hp" as (?) "(_ & _ & >Ho3')".
-        iApply excl_falso. iFrame.
-      + iDestruct "Hp" as (f x) "(>Hp & Hs')".
-        wp_load. iMod ("Hclose" with "[-Ho3 HΦ Hhd]").
-        { iNext. iFrame. iExists xs, hd. iFrame. iExists m. iFrame.
-          iDestruct (big_sepM_delete _ m with "[-]") as "?"=>//.
-          iFrame. iExists #p. iSplitR; first auto. iExists (γx, γ1, γ3, γ4, γq), p.
-          iSplitR; first auto. iFrame.
-          iRight. iLeft. iExists f, x. iFrame. }
-        iModIntro. wp_match.
-        wp_bind (try_srv _ _). iApply try_srv_spec=>//.
-        iFrame "#". wp_seq.
-        iAssert (∃ hd, evs γs hd #p)%I with "[Hhd]" as "Hhd"; eauto.
-        by iApply ("IH" with "Ho3 Hhd").
-      + iDestruct "Hp" as (f x) "(Hp & Hx & Ho2 & Ho4)".
-        wp_load.
-        iMod ("Hclose" with "[-Ho3 HΦ Hhd]").
-        { iNext. iFrame. iExists xs, hd. iFrame. iExists m. iFrame.
-          iDestruct (big_sepM_delete _ m with "[-]") as "?"=>//.
-          iFrame. iExists #p. iSplitR; auto. iExists (γx, γ1, γ3, γ4, γq), p.
-          iSplitR; first auto. iFrame.
-          iRight. iRight. iLeft. iExists f, x. iFrame. }
-        iModIntro. wp_match.
-        wp_bind (try_srv _ _). iApply try_srv_spec=>//.
-        iFrame "#". wp_seq.
-        iAssert (∃ hd, evs γs hd #p)%I with "[Hhd]" as "Hhd"; eauto.
-        by iApply ("IH" with "Ho3 Hhd").
-       + iDestruct "Hp" as (x y) "[>Hp Hs']". iDestruct "Hs'" as (Q) "(>Hx & HoQ & HQ & >Ho1 & >Ho4)".
-          wp_load. iMod ("Hclose" with "[-Ho4 HΦ Hx HoQ HQ]").
-          { iNext. iFrame. iExists xs, hd. iFrame. iExists m. iFrame.
-            iDestruct (big_sepM_delete _ m with "[-]") as "?"=>//.
-            iFrame. iExists #p. iSplitR; auto. iExists (γx, γ1, γ3, γ4, γq), p.
-            iSplitR; first auto. iFrame.
-            iLeft. iExists y. iFrame. }
-          iModIntro. wp_match. iApply ("HΦ" with "[-]"). iFrame.
-          iExists Q. iFrame.
-    - iExFalso. iApply (map_agree_none' _ _ _ m)=>//. iFrame "Hom".
-      rewrite /ev. eauto.
+    wp_bind (! _)%E. iInv N as "Hp" "Hclose".
+    destruct ts as [[[[γx γ1] γ3] γ4] γq].
+    iDestruct "Hp" as "[Hp | [Hp | [ Hp | Hp]]]".
+    + iDestruct "Hp" as (?) "(_ & _ & >Ho3')".
+      iApply excl_falso. iFrame.
+    + iDestruct "Hp" as (f x) "(>Hp & Hs')".
+      wp_load. iMod ("Hclose" with "[Hp Hs']").
+      { iNext. iFrame. iRight. iLeft. iExists f, x. iFrame. }
+      iModIntro. wp_match. wp_bind (try_srv _ _). iApply try_srv_spec=>//.
+      iFrame "#". wp_seq. iApply ("IH" with "Ho3"); eauto.
+    + iDestruct "Hp" as (f x) "(Hp & Hx & Ho2 & Ho4)".
+      wp_load. iMod ("Hclose" with "[-Ho3 HΦ]").
+      { iNext. iFrame. iRight. iRight. iLeft. iExists f, x. iFrame. }
+      iModIntro. wp_match.
+      wp_bind (try_srv _ _). iApply try_srv_spec=>//.
+      iFrame "#". wp_seq. iApply ("IH" with "Ho3"); eauto.
+    + iDestruct "Hp" as (x y) "[>Hp Hs']".
+      iDestruct "Hs'" as (Q) "(>Hx & HoQ & HQ & >Ho1 & >Ho4)".
+      wp_load. iMod ("Hclose" with "[-Ho4 HΦ Hx HoQ HQ]").
+      { iNext. iFrame. iLeft. iExists y. iFrame. }
+      iModIntro. wp_match. iApply ("HΦ" with "[-]"). iFrame.
+      iExists Q. iFrame.
   Qed.
 
-  Lemma mk_flat_spec: mk_syncer_spec mk_flat.
+  Lemma mk_flat_spec (γm: gname): mk_syncer_spec mk_flat.
   Proof.
     iIntros (R Φ) "HR HΦ".
     iMod (own_alloc (Excl ())) as (γr) "Ho2"; first done.
-    iMod (own_alloc (● (∅: tokmR) ⋅ ◯ ∅)) as (γm) "[Hm _]"; first by rewrite -auth_both_op.
-    iAssert (srv_tokm_inv γm) with "[Hm]" as "Hm"; first eauto.
-    { iExists ∅. iFrame. by rewrite big_sepM_empty. }
     wp_seq. wp_bind (newlock _).
     iApply (newlock_spec _ (own γr (Excl ()) ∗ R)%I with "[$Ho2 $HR]")=>//.
     iNext. iIntros (lk γlk) "#Hlk".
     wp_let. wp_bind (new_stack _).
-    iApply (new_stack_spec' _ (p_inv _ γm γr))=>//.
-    iFrame "Hm". iIntros (γ s) "#Hss".
+    iApply (new_bag_spec N (p_inv' R γm γr))=>//.
+    iNext. iIntros (s) "#Hss".
     wp_let. iApply "HΦ". rewrite /synced.
-    iAlways.
-    iIntros (f). wp_let. iAlways.
+    iAlways. iIntros (f). wp_let. iAlways.
     iIntros (P Q x) "#Hf".
-    iIntros "!# Hp". wp_let.
-    wp_bind (install _ _ _).
-    iApply (install_spec R P Q)=>//.
-    iFrame "#". iFrame "Hp". iSplitR; first iApply "Hf".
-    iIntros (p [[[[γx γ1] γ3] γ4] γq]) "(Ho3 & Hx & HoQ) Hev Hhd".
+    iIntros "!# Hp". wp_let. wp_bind (install _ _ _).
+    iApply (install_spec R P Q f x γm γr s with "[-]")=>//.
+    { iFrame. iFrame "#". eauto. }
+    iNext. iIntros (p [[[[γx γ1] γ3] γ4] γq]) "[(Ho3 & Hx & HoQ) #?]".
     wp_let. wp_bind (loop _ _ _).
-    iApply loop_spec=>//.
-    iFrame "#". iFrame.
-    iIntros (? ?) "Hs".
+    iApply (loop_spec with "[-Hx HoQ]")=>//.
+    { iFrame "#". iFrame. }
+    iNext. iIntros (? ?) "Hs".
     iDestruct "Hs" as (Q') "(Hx' & HoQ' & HQ')".
     destruct (decide (x = a)) as [->|Hneq].
     - iDestruct (saved_prop_agree with "[HoQ HoQ']") as "Heq"; first by iFrame.
